common/PrintAST.ml
@@ -41,12 +41,6 @@ let name_of_external = function
   | EF_builtin(name, sg) -> sprintf "builtin %S" (extern_atom name)
   | EF_vload chunk -> sprintf "volatile load %s" (name_of_chunk chunk)
   | EF_vstore chunk -> sprintf "volatile store %s" (name_of_chunk chunk)
-  | EF_vload_global(chunk, id, ofs) ->
-      sprintf "volatile load %s global %S %ld"
-              (name_of_chunk chunk) (extern_atom id) (camlint_of_coqint ofs)
-  | EF_vstore_global(chunk, id, ofs) ->
-      sprintf "volatile store %s global %S %ld"
-              (name_of_chunk chunk) (extern_atom id) (camlint_of_coqint ofs)
   | EF_malloc -> "malloc"
   | EF_free -> "free"
   | EF_memcpy(sz, al) ->
@@ -54,28 +48,38 @@ let name_of_external = function
   | EF_annot(text, targs) -> sprintf "annot %S" (extern_atom text)
   | EF_annot_val(text, targ) ->  sprintf "annot_val %S" (extern_atom text)
   | EF_inline_asm(text, sg, clob) -> sprintf "inline_asm %S" (extern_atom text)
+  | EF_debug(kind, text, targs) ->
+      sprintf "debug%d %S" (P.to_int kind) (extern_atom text)
 
-let rec print_annot_arg px oc = function
-  | AA_base x -> px oc x
-  | AA_int n -> fprintf oc "int %ld" (camlint_of_coqint n)
-  | AA_long n -> fprintf oc "long %Ld" (camlint64_of_coqint n)
-  | AA_float n -> fprintf oc "float %F" (camlfloat_of_coqfloat n)
-  | AA_single n -> fprintf oc "single %F" (camlfloat_of_coqfloat32 n)
-  | AA_loadstack(chunk, ofs) -> 
+let rec print_builtin_arg px oc = function
+  | BA x -> px oc x
+  | BA_int n -> fprintf oc "int %ld" (camlint_of_coqint n)
+  | BA_long n -> fprintf oc "long %Ld" (camlint64_of_coqint n)
+  | BA_float n -> fprintf oc "float %F" (camlfloat_of_coqfloat n)
+  | BA_single n -> fprintf oc "single %F" (camlfloat_of_coqfloat32 n)
+  | BA_loadstack(chunk, ofs) -> 
       fprintf oc "%s[sp + %ld]" (name_of_chunk chunk) (camlint_of_coqint ofs)
-  | AA_addrstack(ofs) ->
+  | BA_addrstack(ofs) ->
       fprintf oc "sp + %ld" (camlint_of_coqint ofs)
-  | AA_loadglobal(chunk, id, ofs) -> 
+  | BA_loadglobal(chunk, id, ofs) -> 
       fprintf oc "%s[&%s + %ld]"
               (name_of_chunk chunk) (extern_atom id) (camlint_of_coqint ofs)
-  | AA_addrglobal(id, ofs) ->
+  | BA_addrglobal(id, ofs) ->
       fprintf oc "&%s + %ld" (extern_atom id) (camlint_of_coqint ofs)
-  | AA_longofwords(hi, lo) ->
-      fprintf oc "longofwords(%a, %a)" 
-                 (print_annot_arg px) hi (print_annot_arg px) lo
+  | BA_longofwords(hi, lo) ->
+      fprintf oc "long(%a, %a)" 
+                 (print_builtin_arg px) hi (print_builtin_arg px) lo
 
-let rec print_annot_args px oc = function
+let rec print_builtin_args px oc = function
   | [] -> ()
-  | [a] -> print_annot_arg px oc a
+  | [a] -> print_builtin_arg px oc a
   | a1 :: al ->
-      fprintf oc "%a, %a" (print_annot_arg px) a1 (print_annot_args px) al
+      fprintf oc "%a, %a" (print_builtin_arg px) a1 (print_builtin_args px) al
+
+let rec print_builtin_res px oc = function
+  | BR x -> px oc x
+  | BR_none -> fprintf oc "_"
+  | BR_longofwords(hi, lo) ->
+      fprintf oc "long(%a, %a)" 
+                 (print_builtin_res px) hi (print_builtin_res px) lo
+
