ia32/Asmexpand.ml
@@ -59,57 +59,21 @@ let sp_adjustment sz =
 (* Handling of annotations *)
 
 let expand_annot_val txt targ args res =
-  emit (Pannot (EF_annot(txt,[targ]), List.map (fun r -> AA_base r) args));
+  emit (Pbuiltin (EF_annot(txt,[targ]), args, BR_none));
   match args, res with
-  | [IR src], [IR dst] ->
+  | [BA(IR src)], BR(IR dst) ->
      if dst <> src then emit (Pmov_rr (dst,src))
-  | [FR src], [FR dst] ->
+  | [BA(FR src)], BR(FR dst) ->
      if dst <> src then emit (Pmovsd_ff (dst,src))
   | _, _ -> assert false
 
-			   
-(* Handling of memcpy *)
+(* Translate a builtin argument into an addressing mode *)
 
-(* Unaligned memory accesses are quite fast on IA32, so use large
-   memory accesses regardless of alignment. *)
-
-let expand_builtin_memcpy_small sz al src dst =
-  assert (src = EDX && dst = EAX);
-  let rec copy ofs sz =
-    if sz >= 8 && !Clflags.option_ffpu then begin
-	emit (Pmovq_rm (XMM7,Addrmode (Some src, None, Coq_inl ofs)));
-	emit (Pmovq_mr (Addrmode (Some src, None, Coq_inl ofs),XMM7));
-        copy (Int.add ofs _8) (sz - 8)
-      end else if sz >= 4 then begin
-	emit (Pmov_rm (ECX,Addrmode (Some src, None, Coq_inl ofs)));
-	emit (Pmov_mr (Addrmode (Some src, None, Coq_inl ofs),ECX));
-        copy (Int.add ofs _4) (sz - 4)
-      end else if sz >= 2 then begin
-	emit (Pmovw_rm (ECX,Addrmode (Some src, None, Coq_inl ofs)));
-	emit (Pmovw_mr (Addrmode (Some src, None, Coq_inl ofs),ECX));
-        copy (Int.add ofs _2) (sz - 2)
-      end else if sz >= 1 then begin
-	emit (Pmovb_rm (ECX,Addrmode (Some src, None, Coq_inl ofs)));
-	emit (Pmovb_mr (Addrmode (Some src, None, Coq_inl ofs),ECX));
-        copy (Int.add ofs _1) (sz - 1)
-      end in
-  copy _0 sz
-
-let expand_builtin_memcpy_big sz al src dst =
-  assert (src = ESI && dst = EDI);
-  emit (Pmov_ri (ECX,coqint_of_camlint (Int32.of_int (sz / 4))));
-  emit Prep_movsl;
-  if sz mod 4 >= 2 then emit Pmovsw;
-  if sz mod 2 >= 1 then emit Pmovsb
-
-let expand_builtin_memcpy sz al args =
-  let (dst, src) =
-    match args with [IR d; IR s] -> (d, s) | _ -> assert false in
-  if sz <= 32
-  then expand_builtin_memcpy_small sz al src dst
-  else expand_builtin_memcpy_big sz al src dst
- 	   
-(* Handling of volatile reads and writes *)
+let addressing_of_builtin_arg = function
+  | BA (IR r) -> Addrmode(Some r, None, Coq_inl Integers.Int.zero)
+  | BA_addrstack ofs -> Addrmode(Some ESP, None, Coq_inl ofs)
+  | BA_addrglobal(id, ofs) -> Addrmode(None, None, Coq_inr(id, ofs))
+  | _ -> assert false
 
 let offset_addressing (Addrmode(base, ofs, cst)) delta =
   Addrmode(base, ofs,
@@ -117,19 +81,61 @@ let offset_addressing (Addrmode(base, ofs, cst)) delta =
            | Coq_inl n -> Coq_inl(Integers.Int.add n delta)
            | Coq_inr(id, n) -> Coq_inr(id, Integers.Int.add n delta))
 
+(* Handling of memcpy *)
+
+(* Unaligned memory accesses are quite fast on IA32, so use large
+   memory accesses regardless of alignment. *)
+
+let expand_builtin_memcpy_small sz al src dst =
+  let rec copy src dst sz =
+    if sz >= 8 && !Clflags.option_ffpu then begin
+	emit (Pmovq_rm (XMM7, src));
+	emit (Pmovq_mr (dst, XMM7));
+        copy (offset_addressing src _8) (offset_addressing dst _8) (sz - 8)
+      end else if sz >= 4 then begin
+	emit (Pmov_rm (ECX, src));
+	emit (Pmov_mr (dst, ECX));
+        copy (offset_addressing src _4) (offset_addressing dst _4) (sz - 4)
+      end else if sz >= 2 then begin
+	emit (Pmovw_rm (ECX, src));
+	emit (Pmovw_mr (dst, ECX));
+        copy (offset_addressing src _2) (offset_addressing dst _2) (sz - 2)
+      end else if sz >= 1 then begin
+	emit (Pmovb_rm (ECX, src));
+	emit (Pmovb_mr (dst, ECX));
+        copy (offset_addressing src _1) (offset_addressing dst _1) (sz - 1)
+      end in
+  copy (addressing_of_builtin_arg src) (addressing_of_builtin_arg dst) sz
+
+let expand_builtin_memcpy_big sz al src dst =
+  if src <> BA (IR ESI) then emit (Plea (ESI, addressing_of_builtin_arg src));
+  if dst <> BA (IR EDI) then emit (Plea (EDI, addressing_of_builtin_arg dst));
+  emit (Pmov_ri (ECX,coqint_of_camlint (Int32.of_int (sz / 4))));
+  emit Prep_movsl;
+  if sz mod 4 >= 2 then emit Pmovsw;
+  if sz mod 2 >= 1 then emit Pmovsb
+
+let expand_builtin_memcpy sz al args =
+  let (dst, src) = match args with [d; s] -> (d, s) | _ -> assert false in
+  if sz <= 32
+  then expand_builtin_memcpy_small sz al src dst
+  else expand_builtin_memcpy_big sz al src dst
+ 	   
+(* Handling of volatile reads and writes *)
+
 let expand_builtin_vload_common chunk addr res =
   match chunk, res with
-  | Mint8unsigned, [IR res] ->
+  | Mint8unsigned, BR(IR res) ->
      emit (Pmovzb_rm (res,addr))
-  | Mint8signed, [IR res] ->
+  | Mint8signed, BR(IR res) ->
      emit (Pmovsb_rm (res,addr))
-  | Mint16unsigned, [IR res] ->
+  | Mint16unsigned, BR(IR res) ->
      emit (Pmovzw_rm (res,addr))
-  | Mint16signed, [IR res] ->
+  | Mint16signed, BR(IR res) ->
      emit (Pmovsw_rm (res,addr))
-  | Mint32, [IR res] ->
+  | Mint32, BR(IR res) ->
      emit (Pmov_rm (res,addr))
-  | Mint64, [IR res1; IR res2] ->
+  | Mint64, BR_longofwords(BR(IR res1), BR(IR res2)) ->
      let addr' = offset_addressing addr (coqint_of_camlint 4l) in
      if not (Asmgen.addressing_mentions addr res2) then begin
 	 emit (Pmov_rm (res2,addr));
@@ -138,60 +144,51 @@ let expand_builtin_vload_common chunk addr res =
 	 emit (Pmov_rm (res1,addr'));
 	 emit (Pmov_rm (res2,addr))
        end
-  | Mfloat32, [FR res] ->
+  | Mfloat32, BR(FR res) ->
      emit (Pmovss_fm (res,addr))
-  | Mfloat64, [FR res] ->
+  | Mfloat64, BR(FR res) ->
      emit (Pmovsd_fm (res,addr))
   | _ ->
      assert false
 
 let expand_builtin_vload chunk args res =
   match args with
-  | [IR addr] ->
-     expand_builtin_vload_common chunk (Addrmode (Some addr,None, Coq_inl _0)) res
+  | [addr] ->
+     expand_builtin_vload_common chunk (addressing_of_builtin_arg addr) res
   | _ ->
      assert false
 
-let expand_builtin_vload_global chunk id ofs args res =
-  expand_builtin_vload_common chunk (Addrmode(None, None, Coq_inr(id,ofs))) res
-			      
 let expand_builtin_vstore_common chunk addr src tmp =
   match chunk, src with
-  | (Mint8signed | Mint8unsigned), [IR src] ->
+  | (Mint8signed | Mint8unsigned), BA(IR src) ->
      if Asmgen.low_ireg src then
        emit (Pmovb_mr (addr,src))
      else begin
 	 emit (Pmov_rr (tmp,src));
 	 emit (Pmovb_mr (addr,tmp))
        end
-  | (Mint16signed | Mint16unsigned), [IR src] ->
+  | (Mint16signed | Mint16unsigned), BA(IR src) ->
      emit (Pmovw_mr (addr,src))
-  | Mint32, [IR src] ->
+  | Mint32, BA(IR src) ->
      emit (Pmov_mr (addr,src))
-  | Mint64, [IR src1; IR src2] ->
+  | Mint64, BA_longofwords(BA(IR src1), BA(IR src2)) ->
      let addr' = offset_addressing addr (coqint_of_camlint 4l) in
      emit (Pmov_mr (addr,src2));
      emit (Pmov_mr (addr',src1))
-  | Mfloat32, [FR src] ->
+  | Mfloat32, BA(FR src) ->
      emit (Pmovss_mf (addr,src))
-  | Mfloat64, [FR src] ->
+  | Mfloat64, BA(FR src) ->
      emit (Pmovsd_mf (addr,src))
   | _ ->
      assert false
 
 let expand_builtin_vstore chunk args =
   match args with
-  | IR addr :: src ->
-     expand_builtin_vstore_common chunk
-       (Addrmode(Some addr, None, Coq_inl Integers.Int.zero)) src
-       (if addr = EAX then ECX else EAX)
+  | [addr; src] ->
+     let addr = addressing_of_builtin_arg addr in
+     expand_builtin_vstore_common chunk addr src
+       (if Asmgen.addressing_mentions addr EAX then ECX else EAX)
   | _ -> assert false
-
-		
-let expand_builtin_vstore_global chunk id ofs args =
-  expand_builtin_vstore_common chunk
-    (Addrmode(None, None, Coq_inr(id,ofs))) args EAX
-
 		 
 (* Handling of varargs *)
 		 
@@ -210,27 +207,27 @@ let expand_builtin_va_start r =
 let expand_builtin_inline name args res =
   match name, args, res with
   (* Integer arithmetic *)
-  | ("__builtin_bswap"| "__builtin_bswap32"), [IR a1], [IR res] ->
+  | ("__builtin_bswap"| "__builtin_bswap32"), [BA(IR a1)], BR(IR res) ->
      if a1 <> res then
        emit (Pmov_rr (res,a1));
      emit (Pbswap res)
-  | "__builtin_bswap16", [IR a1], [IR res] ->
+  | "__builtin_bswap16", [BA(IR a1)], BR(IR res) ->
      if a1 <> res then
        emit (Pmov_rr (res,a1));
      emit (Prolw_8 res)
-  | "__builtin_clz", [IR a1], [IR res] ->
+  | "__builtin_clz", [BA(IR a1)], BR(IR res) ->
      emit (Pbslr (a1,res));
      emit (Pxor_ri(res,coqint_of_camlint 31l))
-  | "__builtin_ctz", [IR a1], [IR res] ->
+  | "__builtin_ctz", [BA(IR a1)], BR(IR res) ->
      emit (Pbsfl (a1,res))
   (* Float arithmetic *)
-  | "__builtin_fabs", [FR a1], [FR res] ->
+  | "__builtin_fabs", [BA(FR a1)], BR(FR res) ->
      if a1 <> res then
        emit (Pmovsd_ff (a1,res));
      emit (Pabsd res) (* This ensures that need_masks is set to true *)
-  | "__builtin_fsqrt", [FR a1], [FR res] ->
+  | "__builtin_fsqrt", [BA(FR a1)], BR(FR res) ->
      emit (Psqrtsd (a1,res))
-  | "__builtin_fmax", [FR a1; FR a2], [FR res] ->
+  | "__builtin_fmax", [BA(FR a1); BA(FR a2)], BR(FR res) ->
      if res = a1 then
        emit (Pmaxsd (a2,res))
      else if res = a2 then
@@ -239,7 +236,7 @@ let expand_builtin_inline name args res =
 	 emit (Pmovsd_ff (a1,res));
 	 emit (Pmaxsd (a2,res))
        end
-  | "__builtin_fmin", [FR a1; FR a2], [FR res] ->
+  | "__builtin_fmin", [BA(FR a1); BA(FR a2)], BR(FR res) ->
      if res = a1 then
        emit (Pminsd (a2,res))
      else if res = a2 then
@@ -248,7 +245,7 @@ let expand_builtin_inline name args res =
 	 emit (Pmovsd_ff (a1,res));
 	 emit (Pminsd (a2,res))
        end
-  | "__builtin_fmadd",  [FR a1; FR a2; FR a3], [FR res] ->
+  | "__builtin_fmadd",  [BA(FR a1); BA(FR a2); BA(FR a3)], BR(FR res) ->
      if res = a1 then
        emit (Pfmadd132 (a2,a3,res))
      else if res = a2 then
@@ -259,7 +256,7 @@ let expand_builtin_inline name args res =
 	 emit (Pmovsd_ff (a2,res));
 	 emit (Pfmadd231 (a1,a2,res))
        end
-  |"__builtin_fmsub",  [FR a1; FR a2; FR a3], [FR res] ->
+  |"__builtin_fmsub",  [BA(FR a1); BA(FR a2); BA(FR a3)], BR(FR res) ->
      if res = a1 then
        emit (Pfmsub132 (a2,a3,res))
      else if res = a2 then
@@ -270,7 +267,7 @@ let expand_builtin_inline name args res =
 	 emit (Pmovsd_ff (a2,res));
 	 emit (Pfmsub231 (a1,a2,res))
        end
-  | "__builtin_fnmadd",  [FR a1; FR a2; FR a3], [FR res] ->
+  | "__builtin_fnmadd",  [BA(FR a1); BA(FR a2); BA(FR a3)], BR(FR res) ->
      if res = a1 then
        emit (Pfnmadd132 (a2,a3,res))
      else if res = a2 then
@@ -281,7 +278,7 @@ let expand_builtin_inline name args res =
 	 emit (Pmovsd_ff (a2,res));
 	 emit (Pfnmadd231 (a1,a2,res))
        end
-  |"__builtin_fnmsub",  [FR a1; FR a2; FR a3], [FR res] ->
+  |"__builtin_fnmsub",  [BA(FR a1); BA(FR a2); BA(FR a3)], BR(FR res) ->
      if res = a1 then
        emit (Pfnmsub132 (a2,a3,res))
      else if res = a2 then
@@ -293,32 +290,38 @@ let expand_builtin_inline name args res =
 	 emit (Pfnmsub231 (a1,a2,res))
        end
   (* 64-bit integer arithmetic *)
-  | "__builtin_negl", [IR ah; IR al], [IR rh; IR rl] ->
+  | "__builtin_negl", [BA_longofwords(BA(IR ah), BA(IR al))],
+                      BR_longofwords(BR(IR rh), BR(IR rl)) ->
      assert (ah = EDX && al = EAX && rh = EDX && rl = EAX);
      emit (Pneg EAX);
      emit (Padcl_ir (_0,EDX));
      emit (Pneg EDX)
-  | "__builtin_addl", [IR ah; IR al; IR bh; IR bl], [IR rh; IR rl] ->
+  | "__builtin_addl", [BA_longofwords(BA(IR ah), BA(IR al));
+                       BA_longofwords(BA(IR bh), BA(IR bl))],
+                       BR_longofwords(BR(IR rh), BR(IR rl)) ->
      assert (ah = EDX && al = EAX && bh = ECX && bl = EBX && rh = EDX && rl = EAX);
      emit (Paddl (EBX,EAX));
      emit (Padcl_rr (ECX,EDX))
-  | "__builtin_subl", [IR ah; IR al; IR bh; IR bl], [IR rh; IR rl] ->
+  | "__builtin_subl", [BA_longofwords(BA(IR ah), BA(IR al));
+                       BA_longofwords(BA(IR bh), BA(IR bl))],
+                       BR_longofwords(BR(IR rh), BR(IR rl)) ->
      assert (ah = EDX && al = EAX && bh = ECX && bl = EBX && rh = EDX && rl = EAX);
      emit (Psub_rr (EBX,EAX));
      emit (Psbbl (ECX,EDX))
-  | "__builtin_mull", [IR a; IR b], [IR rh; IR rl] ->
+  | "__builtin_mull", [BA(IR a); BA(IR b)],
+                      BR_longofwords(BR(IR rh), BR(IR rl)) ->
      assert (a = EAX && b = EDX && rh = EDX && rl = EAX);
      emit (Pmul_r EDX)
   (* Memory accesses *)
-  | "__builtin_read16_reversed", [IR a1], [IR res] ->
+  | "__builtin_read16_reversed", [BA(IR a1)], BR(IR res) ->
      let addr = Addrmode(Some a1,None,Coq_inl _0) in
      emit (Pmovzw_rm (res,addr));
      emit (Prolw_8 res)
-  | "__builtin_read32_reversed", [IR a1], [IR res] ->
+  | "__builtin_read32_reversed", [BA(IR a1)], BR(IR res) ->
      let addr = Addrmode(Some a1,None,Coq_inl _0) in
      emit (Pmov_rm (res,addr));
      emit (Pbswap res)
-  | "__builtin_write16_reversed", [IR a1; IR a2], _ ->
+  | "__builtin_write16_reversed", [BA(IR a1); BA(IR a2)], _ ->
      let tmp = if a1 = ECX then EDX else ECX in
      let addr = Addrmode(Some a1,None,Coq_inl _0) in
      if a2 <> tmp then
@@ -326,7 +329,7 @@ let expand_builtin_inline name args res =
      emit (Pxchg (tmp,tmp));
      emit (Pmovw_mr (addr,tmp))
   (* Vararg stuff *)
-  | "__builtin_va_start", [IR a], _ ->
+  | "__builtin_va_start", [BA(IR a)], _ ->
      expand_builtin_va_start a
   (* Synchronization *)
   | "__builtin_membar", [], _ ->
@@ -335,7 +338,7 @@ let expand_builtin_inline name args res =
   | _ ->
      invalid_arg ("unrecognized builtin " ^ name)
 
-
+(* Expansion of instructions *)
        
 let expand_instruction instr =
   match instr with
@@ -361,18 +364,15 @@ let expand_instruction instr =
           expand_builtin_vload chunk args res
        | EF_vstore chunk ->
           expand_builtin_vstore chunk args
-       | EF_vload_global(chunk, id, ofs) ->
-          expand_builtin_vload_global chunk id ofs args res
-       | EF_vstore_global(chunk, id, ofs) ->
-          expand_builtin_vstore_global chunk id ofs args
        | EF_memcpy(sz, al) ->
           expand_builtin_memcpy (Int32.to_int (camlint_of_coqint sz))
 	    (Int32.to_int (camlint_of_coqint al)) args
        | EF_annot_val(txt, targ) ->
           expand_annot_val txt targ args res      
-       | EF_inline_asm(txt, sg, clob) ->
+       | EF_annot _ | EF_debug _ | EF_inline_asm _ ->
           emit instr
-       | _ -> assert false
+       | _ ->
+          assert false
      end
   | _ -> emit instr
        
