backend/CleanupLabelsproof.v
@@ -291,15 +291,11 @@ Proof.
   econstructor; eauto.
 (* Lbuiltin *)
   left; econstructor; split.
-  econstructor; eauto. eapply external_call_symbols_preserved'; eauto.
-  exact symbols_preserved.  exact public_preserved. exact varinfo_preserved.
-  econstructor; eauto with coqlib.
-(* Lannot *)
-  left; econstructor; split.
-  econstructor; eauto. 
-  eapply eval_annot_args_preserved with (ge1 := ge); eauto. exact symbols_preserved.
+  econstructor.
+  eapply eval_builtin_args_preserved with (ge1 := ge); eauto. exact symbols_preserved.
   eapply external_call_symbols_preserved; eauto.
   exact symbols_preserved.  exact public_preserved. exact varinfo_preserved.
+  eauto.
   econstructor; eauto with coqlib.
 (* Llabel *)
   case_eq (Labelset.mem lbl (labels_branched_to (fn_code f))); intros.
