backend/Linearizeproof.v
@@ -644,14 +644,7 @@ Proof.
   (* Lbuiltin *)
   left; econstructor; split. simpl.
   apply plus_one. eapply exec_Lbuiltin; eauto.
-  eapply external_call_symbols_preserved'; eauto.
-  exact symbols_preserved. exact public_preserved. exact varinfo_preserved.
-  econstructor; eauto.
-
-  (* Lannot *)
-  left; econstructor; split. simpl.
-  apply plus_one. eapply exec_Lannot; eauto.
-  eapply eval_annot_args_preserved with (ge1 := ge); eauto. exact symbols_preserved.
+  eapply eval_builtin_args_preserved with (ge1 := ge); eauto. exact symbols_preserved.
   eapply external_call_symbols_preserved; eauto.
   exact symbols_preserved. exact public_preserved. exact varinfo_preserved.
   econstructor; eauto.
