ia32/Asmgen.v
@@ -536,9 +536,7 @@ Definition transl_instr (f: Mach.function) (i: Mach.instruction)
       OK (Pfreeframe f.(fn_stacksize) f.(fn_retaddr_ofs) f.(fn_link_ofs) :: 
           Pret :: k)
   | Mbuiltin ef args res =>
-      OK (Pbuiltin ef (List.map preg_of args) (List.map preg_of res) :: k)
-  | Mannot ef args =>
-      OK (Pannot ef (List.map (map_annot_arg preg_of) args) :: k)
+      OK (Pbuiltin ef (List.map (map_builtin_arg preg_of) args) (map_builtin_res preg_of res) :: k)
   end.
 
 (** Translation of a code sequence *)
